\documentclass{article}
\usepackage{epsfig}
\pagestyle{empty}
\begin{document}
$ t = 0 $
\pagebreak

\[ \int_S \zeta(\vec{x})\,dA = \int_{S} \zeta_G(\vec{x})\,dA - C = 0, \]
\pagebreak

$ \zeta_G $
\pagebreak

$ B_n(x) $
\pagebreak

$ B_0(x) $
\pagebreak

$ B_1(x) $
\pagebreak

$ \frac{1}{A} \int f(x)\, dA $
\pagebreak

$ \delta(x,y,0) $
\pagebreak

$ \zeta(x,y,0) $
\pagebreak

$ \vec{u}(x,y,0) $
\pagebreak

$ h(x,y,0) $
\pagebreak

$ h_B(x,y) $
\pagebreak

$ (x(t),y(t),z(t)) $
\pagebreak

$ (x_0, y_0, z_0) $
\pagebreak

$ \zeta(\vec{x},t) $
\pagebreak

$ \vec{u}(\vec{x},t) $
\pagebreak

$ \psi(\vec{x},t) $
\pagebreak

\begin{align*} \frac{\partial \zeta}{\partial t} + \vec{u}\cdot\nabla \zeta & = \frac{D\zeta}{Dt} = 0, \\ \nabla^2 \psi & = - \zeta, \\ \zeta &= \nabla \times \vec{u}. \end{align*}
\pagebreak

$ \zeta(x,y,t) $
\pagebreak

$ \delta(x,y,t) $
\pagebreak

$ q(x_0,y_0) $
\pagebreak

$ \vec{u}(x,y,t) $
\pagebreak

$ h(x,y,t) $
\pagebreak

$ \eta_B(x,y) $
\pagebreak

\begin{align} q &= \frac{\zeta + f}{h}, \\ \eta &= \eta_B + h, \end{align}
\pagebreak

$ f = f_0 + \beta y(t) $
\pagebreak

$ f_0 $
\pagebreak

$ \beta $
\pagebreak

$ \eta $
\pagebreak

\begin{align*} \vec{u}(\vec{x},t) &= \int_{\mathbb{R}^2} \left(\vec{K}_\zeta(\vec{x},\vec{y})\zeta(\vec{y}) + \vec{K}_\delta(\vec{x},\vec{y})\delta(\vec{y})\right)\, dA(\vec{y}), \\ \frac{d\vec{x}}{dt} &= \vec{u}(\vec{x},t), \\ \frac{d\zeta}{dt} &= -\beta \frac{dy}{dt} - (\zeta + f)\delta, \\ \frac{d\delta}{dt} &= f\zeta -\vec{u}\cdot(\nabla\times f\vec{k}) - \nabla\vec{u}:\nabla\vec{u} - g\nabla^2 \eta, \\ \frac{dh}{dt} &= -h\delta, \\ \frac{dA}{dt} &= \delta A, \end{align*}
\pagebreak

$ \vec{K}_\zeta = -\nabla \times G $
\pagebreak

$ \vec{K}_\delta = \nabla G $
\pagebreak

\[ G(\vec{x},\vec{y}) = \frac{1}{4\pi}\log( |\vec{x}-\vec{y}|^2). \]
\pagebreak

$ \nabla\vec{u}:\nabla\vec{u}$
\pagebreak

$ \vec{K}_\zeta $
\pagebreak

$ \vec{K}_\delta $
\pagebreak

$ D = \{ (x,y) : x,y\in [-1,1] \} $
\pagebreak

$p_i$
\pagebreak

$ e_i $
\pagebreak

$ F_i $
\pagebreak

$ \epsilon $
\pagebreak

$ \Delta x $
\pagebreak

\[ \epsilon = \Delta x^{1/p},\quad p>1. \]
\pagebreak

$ D^\beta $
\pagebreak

$ L^\beta $
\pagebreak

\[ D^\beta f(\vec{x}) \approx L^\beta f(\vec{x}) = \frac{1}{\epsilon^{|\beta|}}\int_{\mathbb{R}^d} \left( f(\vec{y}) \mp f(\vec{x})\right)\eta_\epsilon^\beta(\vec{x}-\vec{y})\,dV(\vec{y}), \]
\pagebreak

$ \eta_{\epsilon}^\beta = \eta^\beta(|\vec{x}|/\epsilon) $
\pagebreak

$\eta^\beta $
\pagebreak

$D^\beta$
\pagebreak

$ \epsilon\to 0$
\pagebreak

\[ \epsilon = \Delta x^{1/p},\quad p > 1 \]
\pagebreak

$ \frac{|\vec{x}_i - \vec{x}_j|}{\epsilon} $
\pagebreak

$ \mathbb{R}^2 $
\pagebreak

$ \int_{F_i} f(x)\,dx \approx $
\pagebreak

$ \max_{F_i} f(x) - \min_{F_i} f(x) $
\pagebreak

$ \sum_{i=1}^3 \left(\max_{F_j} x0_i - \min_{F_j} x0_i\right) $
\pagebreak

$ \zeta(x,y,z,t) $
\pagebreak

$ \omega(x_0,y_0,z_0) $
\pagebreak

\[ \omega = \zeta + f, \]
\pagebreak

$ f = \frac{2\Omega}{a}z(t) $
\pagebreak

$ \Omega $
\pagebreak

$ a $
\pagebreak

$ \psi_r(x,y,z,t) $
\pagebreak

$ \psi_a(x,y,z,t) $
\pagebreak

\begin{align*} \psi_r(\vec{x},t) &= \frac{1}{4\pi a}\int_{S} \log( 1 - \vec{x} \cdot \vec{\tilde{x}})\zeta(\vec{\tilde{x}})\,dA, \\ \psi_a(\vec{x},t) &= \frac{1}{4\pi a}\int_{S} \log( 1 - \vec{x} \cdot \vec{\tilde{x}})\omega(\vec{\tilde{x}})\,dA. \end{align*}
\pagebreak

\[ \vec{u}(\vec{x},t) = -\frac{1}{4\pi a}\int_{S} \frac{ \vec{x} \times \vec{\tilde{x}} }{a^2 - \vec{x}\cdot\vec{\tilde{x}}} \zeta(\vec{\tilde{x}})\,dA. \]
\pagebreak

$ P = I - x x^T $
\pagebreak

$ x_A \cdot (x_b \times x_c) $
\pagebreak

$\vec{u}$
\pagebreak

$ \nabla\vec{u}:\nabla\vec{u} $
\pagebreak

\end{document}
